src/Approx.v
@@ -1,0 +1,56 @@
+Require Import RelationClasses.
+Require Import ExtLib.Structures.Monads.
+
+Set Implicit Arguments.
+Set Strict Implicit.
+
+Section approx.
+  Variable T : Type.
+  Variable f : (T -> T * bool) -> T -> T * bool.
+  
+  Fixpoint approx (x : T) (fuel : nat) : T * bool :=
+    match fuel with
+      | 0 => (x,false)
+      | S fuel => 
+        f (fun z => approx z fuel) x
+    end.
+
+  Section relational.
+    Variable P : T -> T -> Prop.
+    Hypothesis Refl_P : Reflexive P.
+    Hypothesis Trans_P : Transitive P.
+    Hypothesis related : forall F, (forall y, P y (fst (F y))) -> forall x, P x (fst (f F x)).
+
+    Theorem approx_preserves : forall n x,
+                                   P x (fst (approx x n)).
+    Proof.
+      induction n; simpl; intros; auto.
+    Qed.
+  End relational.
+
+End approx.
+    
+Section approx2.
+  Variable T : Type.
+  Variable stop : T -> T -> bool.
+  Variable f : T -> T.
+  
+  Definition approx2 (x : T) (fuel : nat) : T :=
+    fst (approx (fun F x => let x' := f x in
+                            if stop x x' then (x,false) else F x') x fuel).
+
+  Variable P : T -> Prop.
+  Hypothesis preserves : forall x, P x -> P (f x).
+
+  Lemma approx2_preserves : forall n x, 
+                              P x -> 
+                              P (approx2 x n).
+  Proof.
+    unfold approx2.
+    intros. revert H. eapply approx_preserves; auto; intros.
+    destruct (stop x0 (f x0)); simpl; auto.    
+  Qed.
+End approx2.
+        
+          
+    
