src/MonadReduceApprox.v
@@ -1,0 +1,105 @@
+Require Import List Bool.
+Require Import ExtLib.Core.Type.
+Require Import ExtLib.Structures.Monads.
+Require Import ExtLib.Data.Fun.
+Require Import ExtLib.Data.Vector.
+Require Import ExtLib.Data.Monads.FuelMonad.
+Require Import ExtLib.Relations.TransitiveClosure.
+Require Import ExtLib.Recur.Relation.
+Require Import MirrorCore.TypesExt.
+Require Import MirrorCore.ExprExt.
+
+Set Implicit Arguments.
+Set Strict Implicit.
+
+Section Demo.
+
+  Variable m : Type -> Type.
+  Context {Monad_m : Monad m}.
+
+  Variable typ : Type.
+  Variable typD : list Type -> typ -> Type.
+  Variable expr : Type.
+  Context {Expr_expr : Expr typD expr}.
+  Context {RType_typ : RType typD}.
+  Context {RTypeOk_typ : RTypeOk RType_typ}.
+  Context {typ_arr : TypInstance2 typD Fun}.
+  Context {typ_m : TypInstance1 typD m}.
+  Let tvArr := @typ2 _ typD _ typ_arr.
+  Let tvM := @typ1 _ typD _ typ_m.
+
+  Variable bind_app : @SymAppN typ _ expr _ 2 ((fun x => tvM (vector_hd x)) :: (fun x => tvArr (vector_hd x) (tvM (vector_hd (vector_tl x)))):: nil) (fun _ => tvM).
+  Variable ret_app : @SymAppN typ _ expr _ 1 (vector_hd :: nil) tvM.
+  Variable app_i : forall d r, @AppInstance _ typD expr _ (tvArr d r) d r.
+  Variable lam : @Lambda typ _ expr _.
+
+  Let Bind (t1 t2 : typ) (b1 b2 : expr) : expr := 
+    sappn bind_app (Vcons t1 (Vcons t2 (Vnil _)))
+                   (Vcons b1 (Vcons b2 (Vnil _))).
+  Let Ret (t1 : typ) (b1 : expr) : expr := 
+    sappn ret_app (Vcons t1 (Vnil _))
+                  (Vcons b1 (Vnil _)).
+
+  Definition monad_match (R : Type) (e : expr) 
+             (caseRet : typ -> forall e' : expr, acc e' e -> R)
+             (caseBind : typ -> typ -> forall e' e'' : expr, acc e' e -> acc e'' e -> R)
+             (caseElse : unit -> R) : R.
+  refine (
+    match sappn_check bind_app e with
+      | Some (existT vs_es pf) => 
+        caseBind (vector_hd (fst vs_es)) (vector_hd (vector_tl (fst vs_es)))
+                 (vector_hd (snd vs_es)) (vector_hd (vector_tl (snd vs_es)))
+                 _ _
+      | None => match sappn_check ret_app e with
+                  | Some (existT vs_es _) => 
+                    caseRet (vector_hd (fst vs_es)) (vector_hd (snd vs_es))
+                            _
+                  | None => caseElse tt
+                end
+    end); repeat (eassumption || apply ForallV_vector_hd || apply ForallV_vector_tl).
+  Defined.
+
+  Require Import MirrorCore.Approx.
+
+  Definition monad_red (recur : expr -> expr * bool) (e : expr) : expr * bool :=
+    let do_lam e := 
+        match lambda_check lam e with
+          | None => inl e
+          | Some (existT (t,e) _) => 
+            match recur e with
+              | (e',true) => inr (t,e')
+              | (e',false) => inl e
+            end                       
+        end
+    in
+    @monad_match (expr * bool) e
+                 (fun _ _ _ => (e, false))
+                 (fun t1 t2 b1 b2 _ _ =>
+                    let b1' := recur b1 in
+                    match sappn_check ret_app (fst b1') with
+                      | None => 
+                        let b2' := do_lam b2 in
+                        match b2' with
+                          | inl b2' => (Bind t1 t2 (fst b1') b2, snd b1')
+                          | inr (t,b2') => (Bind t1 t2 (fst b1') (lambda lam t b2'), true)
+                        end
+                      | Some (existT (t, v) _) =>
+                        let t := vector_hd t in
+                        let v := vector_hd v in
+                        let b2' := do_lam b2 in
+                        match b2' with
+                          | inl b2' => 
+                            (@app1 _ typD expr _ _ _ _ (app_i t (tvM t2)) b2' v, true)
+                          | inr (_, b2') =>
+                            (subst0 lam b2' v, true)
+                        end
+                    end)
+                 (fun _ => (e, false)).
+
+  Definition monad_run' : expr -> nat -> expr * bool :=
+    @approx _ monad_red.
+
+  Definition monad_run (e : expr) : expr :=
+    fst (monad_run' e 100).    
+
+End Demo.
